Assignment 12 and others

sf/Assignment12_05.v
@@ -4,47 +4,73 @@ Require Export Assignment12_04.
 
 (** Translate this informal recursive definition into one using [fix]:
 <<
-   halve = 
-     \x:Nat. 
-        if x=0 then 0 
+   halve =
+     \x:Nat.
+        if x=0 then 0
         else if (pred x)=0 then 0
         else 1 + (halve (pred (pred x))))
 >>
 *)
 
 Definition halve : tm :=
-  FILL_IN_HERE.
+  tfix
+    (tabs A (TArrow TNat TNat)
+      (tabs B TNat
+        (tif0 (tvar B)
+           (tnat 0)
+           (tif0 (tpred (tvar B))
+             (tnat 0)
+             (tsucc (tapp (tvar A) (tpred (tpred (tvar B)))))
+           )
+        )
+      )
+    ).
 
 Example halve_type: empty |- halve \in TArrow TNat TNat.
 Proof.
-  (* unfold halve; eauto 10. *)
-  exact FILL_IN_HERE.
+  unfold halve; eauto 10.
 Qed.
 
 Example halve_10: tapp halve (tnat 10) ==>* tnat 5.
 Proof.
-  (* unfold halve; normalize. *)
-  exact FILL_IN_HERE.
+  unfold halve; normalize.
 Qed.
 
 Example halve_11: tapp halve (tnat 11) ==>* tnat 5.
 Proof.
-  (* unfold halve; normalize. *)
-  exact FILL_IN_HERE.
+  unfold halve; normalize.
 Qed.
 
 
 Theorem halve_correct: forall n,
    tapp halve (tnat (n+n)) ==>* tnat n.
-Proof.
-  exact FILL_IN_HERE.
+Proof with eauto.
+  intros.
+  induction n. unfold halve.  normalize.
+
+  apply multi_trans with (y := (tsucc (tapp halve (tnat (n + n))))).
+  unfold halve.
+  eapply multi_step...
+  eapply multi_step...
+  eapply multi_step.
+  apply ST_AppAbs... simpl.
+  eapply multi_step...
+  eapply multi_step... simpl.
+  rewrite <- plus_n_Sm.
+  eapply multi_step...
+  eapply multi_step...
+
+
+
+  apply multi_trans with (y := (tsucc (tnat n)))...
+  induction IHn...
 Qed.
 
 (*-- Check --*)
 
 Check conj halve_type (conj halve_10 halve_11) :
   empty |- halve \in TArrow TNat TNat /\
-  tapp halve (tnat 10) ==>* tnat 5 /\ 
+  tapp halve (tnat 10) ==>* tnat 5 /\
   tapp halve (tnat 11) ==>* tnat 5.
 
 Check halve_correct: forall n,
