sf/Assignment12_01.v
@@ -10,18 +10,28 @@ Require Export Assignment12_00.
 
 Example typing_nonexample_3 :
   ~ (exists S, exists T,
-        empty |- 
+        empty |-
           (tabs X S
              (tapp (tvar X) (tvar X))) \in
           T).
 Proof.
-  exact FILL_IN_HERE.
+  intros not.
+  inversion not. inversion H.
+  inversion H0; subst; clear H0.
+  inversion H6; subst; clear H6.
+  inversion H5; subst; clear H5.
+  inversion H3; subst; clear H3.
+  inversion H2.
+  subst.
+  induction T1; try inversion H4.
+  apply IHT1_1. eapply ex_intro. apply T_Abs.
+  eapply T_App. apply T_Var. rewrite H1. unfold extend. simpl. eauto. auto. auto. rewrite H1.  auto.
 Qed.
 
 (*-- Check --*)
 Check typing_nonexample_3 :
   ~ (exists S, exists T,
-        empty |- 
+        empty |-
           (tabs X S
              (tapp (tvar X) (tvar X))) \in
           T).
