sf/Assignment12_02.v
@@ -3,15 +3,17 @@ Require Export Assignment12_01.
 (* problem #02: 10 points *)
 
 (** **** Exercise: 2 stars, optional (typable_empty__closed)  *)
-Corollary typable_empty__closed : forall t T, 
+Corollary typable_empty__closed : forall t T,
     empty |- t \in T  ->
     closed t.
-Proof.
-  exact FILL_IN_HERE.
+Proof with eauto 12.
+  intros t T HT x x_free.
+  apply free_in_context with (T := T) (Gamma := empty) in x_free; try assumption.
+  inversion x_free as [T' H]. inversion H.
 Qed.
 
 (*-- Check --*)
-Check typable_empty__closed : forall t T, 
+Check typable_empty__closed : forall t T,
     empty |- t \in T  ->
     closed t.
 
