sf/Assignment12_04.v
@@ -3,16 +3,23 @@ Require Export Assignment12_03.
 (* problem #04: 10 points *)
 
 Corollary soundness : forall t t' T,
-  empty |- t \in T -> 
+  empty |- t \in T ->
   t ==>* t' ->
   ~(stuck t').
-Proof.
-  exact FILL_IN_HERE.
+Proof with eauto 12.
+  intros t t' T Hhas_type Hmulti. unfold stuck.
+  intros [Hnf Hnot_val]. unfold normal_form in Hnf.
+  induction Hmulti.
+
+  apply progress in Hhas_type... inversion Hhas_type...
+  apply IHHmulti...
+
+  apply preservation with (t':= y) in Hhas_type...
 Qed.
 
 (*-- Check --*)
 Check soundness : forall t t' T,
-  empty |- t \in T -> 
+  empty |- t \in T ->
   t ==>* t' ->
   ~(stuck t').
 
