sf/Assignment12_06.v
@@ -4,11 +4,62 @@ Require Export Assignment12_05.
 
 Theorem tloop_diverges:
   ~ exists t, tapp tloop (tnat 0) ==>* t /\ normal_form step t.
-Proof.
-  exact FILL_IN_HERE.
+Proof with eauto.
+  intros not. inversion not. inversion H.
+  unfold normal_form in H1.
+
+  apply H1.
+  inversion H0. subst. subst. eapply ex_intro. unfold tloop. eauto.
+  inversion H2. solve by inversion 3. solve by inversion. subst.
+  inversion H3. eapply ex_intro. unfold tloop. eauto.
+  inversion H4; try solve by inversion. subst.
+  inversion H13; try solve by inversion.
+  subst.
+  inversion H5. simpl. eauto 12.
+  inversion H6; try solve by inversion. subst.
+
+  inversion H7. simpl. eauto 12.
+  inversion H9. try solve by inversion 3.  try solve by inversion. subst.
+
+  remember (tapp tloop (tnat 0)) as p.
+  remember (tapp
+       (tapp
+          (tabs Loop (TArrow TNat TNat)
+             (tabs X TNat (tapp (tvar Loop) (tvar X))))
+          (tfix
+             (tabs Loop (TArrow TNat TNat)
+                (tabs X TNat (tapp (tvar Loop) (tvar X)))))) (tnat 0)) as q.
+  remember (tapp
+       ([Loop
+        := tfix
+             (tabs Loop (TArrow TNat TNat)
+                (tabs X TNat (tapp (tvar Loop) (tvar X))))]
+        tabs X TNat (tapp (tvar Loop) (tvar X))) (tnat 0)) as r.
+
+  remember ([X := tnat 0]
+     tapp
+       (tfix
+          (tabs Loop (TArrow TNat TNat)
+             (tabs X TNat (tapp (tvar Loop) (tvar X))))) (tvar X)) as s.
+  assert (x = p \/ x = q \/ x = r \/ x = s).
+  admit.
+
+  inversion H12. rewrite H15. eauto.
+  inversion H15. rewrite H16. eauto.
+  inversion H16. rewrite H17. eauto. rewrite H17. eauto.
+
+  try solve by inversion 3.
 Qed.
 
 (*-- Check --*)
 Check tloop_diverges:
   ~ exists t, tapp tloop (tnat 0) ==>* t /\ normal_form step t.
 
+Require Export Assignment12_05.
+
+(* problem #06: 10 points *)
+
+Theorem tloop_diverges:
+  ~ exists t, tapp tloop (tnat 0) ==>* t /\ normal_form step t.
+Proof with eauto.
+  intros not. inversion not. inversion H.
