sf/Types.v
@@ -2,7 +2,7 @@
 
 Require Export Smallstep.
 
-Hint Constructors multi.  
+Hint Constructors multi.
 
 (** Our next major topic is _type systems_ -- static program
     analyses that classify expressions according to the "shapes" of
@@ -64,7 +64,7 @@ Inductive nvalue : tm -> Prop :=
 Definition value (t:tm) := bvalue t \/ nvalue t.
 
 Hint Constructors bvalue nvalue.
-Hint Unfold value.  
+Hint Unfold value.
 Hint Unfold extend.
 
 (* ###################################################################### *)
@@ -146,9 +146,9 @@ where "t1 '==>' t2" := (step t1 t2).
 
 Tactic Notation "step_cases" tactic(first) ident(c) :=
   first;
-  [ Case_aux c "ST_IfTrue" | Case_aux c "ST_IfFalse" | Case_aux c "ST_If" 
+  [ Case_aux c "ST_IfTrue" | Case_aux c "ST_IfFalse" | Case_aux c "ST_If"
   | Case_aux c "ST_Succ" | Case_aux c "ST_PredZero"
-  | Case_aux c "ST_PredSucc" | Case_aux c "ST_Pred" 
+  | Case_aux c "ST_PredSucc" | Case_aux c "ST_Pred"
   | Case_aux c "ST_IszeroZero" | Case_aux c "ST_IszeroSucc"
   | Case_aux c "ST_Iszero" ].
 
@@ -156,12 +156,12 @@ Hint Constructors step.
 (** Notice that the [step] relation doesn't care about whether
     expressions make global sense -- it just checks that the operation
     in the _next_ reduction step is being applied to the right kinds
-    of operands.  
+    of operands.
 
     For example, the term [succ true] (i.e., [tsucc ttrue] in the
     formal syntax) cannot take a step, but the almost as obviously
     nonsensical term
-       succ (if true then true else true) 
+       succ (if true then true else true)
     can take a step (once, before becoming stuck). *)
 
 (* ###################################################################### *)
@@ -185,7 +185,11 @@ Hint Unfold stuck.
 Example some_term_is_stuck :
   exists t, stuck t.
 Proof.
-  (* FILL IN HERE *) Admitted.
+  exists (tsucc ttrue).
+  unfold stuck.
+  split. unfold normal_form. intros not. inversion not. inversion H. inversion H1.
+  intros not. inversion not. inversion H. inversion H. inversion H1.
+Qed.
 (** [] *)
 
 (** However, although values and normal forms are not the same in this
@@ -205,7 +209,15 @@ Proof.
 Lemma value_is_nf : forall t,
   value t -> step_normal_form t.
 Proof.
-  (* FILL IN HERE *) Admitted.
+  intros.
+  induction H. induction H.
+  unfold normal_form. intros not. inversion not. inversion H.
+  unfold normal_form. intros not. inversion not. inversion H.
+  induction H.
+  unfold normal_form. intros not. inversion not. inversion H.
+  unfold normal_form. intros not. inversion not. unfold normal_form in IHnvalue. apply IHnvalue.
+  inversion H0. subst. inversion H0. subst. exists t1'. apply H4.
+Qed.
 (** [] *)
 
 
@@ -216,7 +228,38 @@ Proof.
 Theorem step_deterministic:
   deterministic step.
 Proof with eauto.
-  (* FILL IN HERE *) Admitted.
+  unfold deterministic. intros x y1 y2 Hy1 Hy2.
+  generalize dependent y2.
+  induction Hy1; intros y2 Hy2.
+  inversion Hy2. reflexivity. inversion H3.
+  inversion Hy2. reflexivity. inversion H3.
+  inversion Hy2. subst. inversion Hy1. subst. inversion Hy1. subst. apply IHHy1 in H3. rewrite H3. eauto.
+  inversion Hy2. subst. inversion Hy2. subst. apply IHHy1 in H2. rewrite H2. eauto.
+  inversion Hy2. reflexivity. inversion H0.
+  assert (value t1). eauto.
+  apply value_is_nf in H0. unfold normal_form in H0.
+  inversion Hy2. reflexivity.
+  subst. inversion H2. subst.
+  exfalso. apply H0. exists t1'0. apply H3.
+  inversion Hy2. subst. inversion Hy1. subst.
+  assert (value y2). eauto.
+  apply value_is_nf in H. unfold normal_form in H.
+  inversion Hy1. subst. exfalso. apply H. eauto.
+  subst. apply IHHy1 in H0. rewrite H0. reflexivity.
+  inversion Hy2. reflexivity. inversion H0.
+  inversion Hy2. reflexivity.
+  assert (value t1). eauto.
+  apply value_is_nf in H3. unfold normal_form in H3.
+
+  inversion H1. subst.
+  exfalso. apply H3. eauto.
+  inversion Hy2. subst. inversion Hy1.
+  subst.
+  assert (value t0). eauto.
+  apply value_is_nf in H. unfold normal_form in H.
+  inversion Hy1. exfalso. apply H. eauto.
+  subst. apply IHHy1 in H0. rewrite H0. reflexivity.
+Qed.
 (** [] *)
 
 
@@ -231,7 +274,7 @@ Proof with eauto.
     _typing relation_ that relates terms to the types (either numeric
     or boolean) of their final results.  *)
 
-Inductive ty : Type := 
+Inductive ty : Type :=
   | TBool : ty
   | TNat : ty.
 
@@ -240,7 +283,7 @@ Inductive ty : Type :=
     called a "turnstile".  (Below, we're going to see richer typing
     relations where an additional "context" argument is written to the
     left of the turnstile.  Here, the context is always empty.) *)
-(** 
+(**
                            ----------------                            (T_True)
                            |- true \in Bool
 
@@ -253,7 +296,7 @@ Inductive ty : Type :=
 
                              ------------                              (T_Zero)
                              |- 0 \in Nat
-                              
+
                             |- t1 \in Nat
                           ------------------                           (T_Succ)
                           |- succ t1 \in Nat
@@ -270,16 +313,16 @@ Inductive ty : Type :=
 Reserved Notation "'|-' t '\in' T" (at level 40).
 
 Inductive has_type : tm -> ty -> Prop :=
-  | T_True : 
+  | T_True :
        |- ttrue \in TBool
-  | T_False : 
+  | T_False :
        |- tfalse \in TBool
   | T_If : forall t1 t2 t3 T,
        |- t1 \in TBool ->
        |- t2 \in T ->
        |- t3 \in T ->
        |- tif t1 t2 t3 \in T
-  | T_Zero : 
+  | T_Zero :
        |- tzero \in TNat
   | T_Succ : forall t1,
        |- t1 \in TNat ->
@@ -308,21 +351,21 @@ Hint Constructors has_type.
     _conservative_ (or _static_) approximation: it does not calculate
     the type of the normal form of a term. *)
 
-Example has_type_1 : 
+Example has_type_1 :
   |- tif tfalse tzero (tsucc tzero) \in TNat.
-Proof. 
-  apply T_If. 
+Proof.
+  apply T_If.
     apply T_False.
     apply T_Zero.
     apply T_Succ.
-      apply T_Zero.  
+      apply T_Zero.
 Qed.
 
 (** (Since we've included all the constructors of the typing relation
     in the hint database, the [auto] tactic can actually find this
     proof automatically.) *)
 
-Example has_type_not : 
+Example has_type_not :
   ~ (|- tif tfalse tzero ttrue \in TBool).
 Proof.
   intros Contra. solve by inversion 2.  Qed.
@@ -330,9 +373,9 @@ Proof.
 (** **** Exercise: 1 star, optional (succ_hastype_nat__hastype_nat)  *)
 Example succ_hastype_nat__hastype_nat : forall t,
   |- tsucc t \in TNat ->
-  |- t \in TNat.  
+  |- t \in TNat.
 Proof.
-  (* FILL IN HERE *) Admitted.
+  intros. inversion H. eauto. Qed.
 (** [] *)
 
 (* ###################################################################### *)
@@ -356,9 +399,9 @@ Lemma nat_canonical : forall t,
 Proof.
   intros t HT HV.
   inversion HV.
-  inversion H; subst; inversion HT.   
+  inversion H; subst; inversion HT.
 
-  auto.  
+  auto.
 Qed.
 
 (* ###################################################################### *)
@@ -391,13 +434,22 @@ Proof with auto.
     SCase "t1 can take a step".
       inversion H as [t1' H1].
       exists (tif t1' t2 t3)...
-  (* FILL IN HERE *) Admitted.
+  Case "T_Succ".
+    inversion IHHT. apply (nat_canonical t1 HT) in H...
+    right. inversion H. exists (tsucc x). eauto.
+  Case "T_Pred".
+    inversion IHHT. apply (nat_canonical t1 HT) in H. inversion H. eauto. eauto.
+    right. inversion H. exists (tpred x). eauto.
+  Case "T_Iszero".
+    inversion IHHT. apply (nat_canonical t1 HT) in H... inversion H. eauto. eauto.
+    right. inversion H. exists (tiszero x). eauto.
+Qed.
 (** [] *)
 
 (** **** Exercise: 3 stars, advanced (finish_progress_informal)  *)
 (** Complete the corresponding informal proof: *)
 
-(** _Theorem_: If [|- t \in T], then either [t] is a value or else 
+(** _Theorem_: If [|- t \in T], then either [t] is a value or else
     [t ==> t'] for some [t']. *)
 
 (** _Proof_: By induction on a derivation of [|- t \in T].
@@ -405,10 +457,10 @@ Proof with auto.
       - If the last rule in the derivation is [T_If], then [t = if t1
         then t2 else t3], with [|- t1 \in Bool], [|- t2 \in T] and [|- t3
         \in T].  By the IH, either [t1] is a value or else [t1] can step
-        to some [t1'].  
+        to some [t1'].
 
             - If [t1] is a value, then by the canonical forms lemmas
-              and the fact that [|- t1 \in Bool] we have that [t1] 
+              and the fact that [|- t1 \in Bool] we have that [t1]
               is a [bvalue] -- i.e., it is either [true] or [false].
               If [t1 = true], then [t] steps to [t2] by [ST_IfTrue],
               while if [t1 = false], then [t] steps to [t3] by
@@ -465,9 +517,9 @@ Theorem preservation : forall t t' T,
 Proof with auto.
   intros t t' T HT HE.
   generalize dependent t'.
-  has_type_cases (induction HT) Case; 
+  has_type_cases (induction HT) Case;
          (* every case needs to introduce a couple of things *)
-         intros t' HE; 
+         intros t' HE;
          (* and we can deal with several impossible
             cases all at once *)
          try (solve by inversion).
@@ -476,7 +528,12 @@ Proof with auto.
       SCase "ST_IfFalse". assumption.
       SCase "ST_If". apply T_If; try assumption.
         apply IHHT1; assumption.
-    (* FILL IN HERE *) Admitted.
+    Case "T_Succ". inversion HE; subst; clear HE. apply T_Succ.
+      apply IHHT. apply H0.
+    Case "T_Pred". inversion HE. eauto. subst. inversion HT. apply H1.
+      subst. inversion HE. eauto. eauto.
+    Case "T_Iszero". inversion HE. eauto. eauto. eauto.
+Qed.
 (** [] *)
 
 (** **** Exercise: 3 stars, advanced (finish_preservation_informal)  *)
@@ -488,7 +545,7 @@ Proof with auto.
 
       - If the last rule in the derivation is [T_If], then [t = if t1
         then t2 else t3], with [|- t1 \in Bool], [|- t2 \in T] and [|- t3
-        \in T].  
+        \in T].
 
         Inspecting the rules for the small-step reduction relation and
         remembering that [t] has the form [if ...], we see that the
@@ -535,12 +592,12 @@ Definition multistep := (multi step).
 Notation "t1 '==>*' t2" := (multistep t1 t2) (at level 40).
 
 Corollary soundness : forall t t' T,
-  |- t \in T -> 
+  |- t \in T ->
   t ==>* t' ->
   ~(stuck t').
-Proof. 
+Proof.
   intros t t' T HT P. induction P; intros [R S].
-  destruct (progress x T HT); auto.   
+  destruct (progress x T HT); auto.
   apply IHP.  apply (preservation x y T HT H).
   unfold stuck. split; auto.   Qed.
 
@@ -557,17 +614,17 @@ Proof.
     relation [astep]. *)
 
 
-Definition amultistep st := multi (astep st). 
+Definition amultistep st := multi (astep st).
 Notation " t '/' st '==>a*' t' " := (amultistep st t t')
   (at level 40, st at level 39).
 
-Example astep_example1 : 
-  (APlus (ANum 3) (AMult (ANum 3) (ANum 4))) / empty_state 
+Example astep_example1 :
+  (APlus (ANum 3) (AMult (ANum 3) (ANum 4))) / empty_state
   ==>a* (ANum 15).
 Proof.
   apply multi_step with (APlus (ANum 3) (ANum 12)).
-    apply AS_Plus2. 
-      apply av_num. 
+    apply AS_Plus2.
+      apply av_num.
       apply AS_Mult.
   apply multi_step with (ANum 15).
     apply AS_Plus.
@@ -580,8 +637,8 @@ Qed.
     them. *)
 
 Hint Constructors astep aval.
-Example astep_example1' : 
-  (APlus (ANum 3) (AMult (ANum 3) (ANum 4))) / empty_state 
+Example astep_example1' :
+  (APlus (ANum 3) (AMult (ANum 3) (ANum 4))) / empty_state
   ==>a* (ANum 15).
 Proof.
   eapply multi_step. auto. simpl.
@@ -596,19 +653,19 @@ Qed.
     evaluated. *)
 
 Tactic Notation "print_goal" := match goal with |- ?x => idtac x end.
-Tactic Notation "normalize" := 
-   repeat (print_goal; eapply multi_step ; 
+Tactic Notation "normalize" :=
+   repeat (print_goal; eapply multi_step ;
              [ (eauto 10; fail) | (instantiate; simpl)]);
    apply multi_refl.
 
 
-Example astep_example1'' : 
-  (APlus (ANum 3) (AMult (ANum 3) (ANum 4))) / empty_state 
+Example astep_example1'' :
+  (APlus (ANum 3) (AMult (ANum 3) (ANum 4))) / empty_state
   ==>a* (ANum 15).
 Proof.
   normalize.
-  (* At this point in the proof script, the Coq response shows 
-     a trace of how the expression evaluated. 
+  (* At this point in the proof script, the Coq response shows
+     a trace of how the expression evaluated.
 
    (APlus (ANum 3) (AMult (ANum 3) (ANum 4)) / empty_state ==>a* ANum 15)
    (multi (astep empty_state) (APlus (ANum 3) (ANum 12)) (ANum 15))
@@ -622,7 +679,7 @@ Qed.
     existential variable in it. *)
 
 Example astep_example1''' : exists e',
-  (APlus (ANum 3) (AMult (ANum 3) (ANum 4))) / empty_state 
+  (APlus (ANum 3) (AMult (ANum 3) (ANum 4))) / empty_state
   ==>a* e'.
 Proof.
   eapply ex_intro. normalize.
@@ -640,10 +697,12 @@ Qed.
 
 (** **** Exercise: 1 star (normalize_ex)  *)
 Theorem normalize_ex : exists e',
-  (AMult (ANum 3) (AMult (ANum 2) (ANum 1))) / empty_state 
+  (AMult (ANum 3) (AMult (ANum 2) (ANum 1))) / empty_state
   ==>a* e'.
 Proof.
-  (* FILL IN HERE *) Admitted.
+  eapply ex_intro.
+  normalize.
+Qed.
 
 (** [] *)
 
@@ -651,10 +710,12 @@ Proof.
 (** For comparison, prove it using [apply] instead of [eapply]. *)
 
 Theorem normalize_ex' : exists e',
-  (AMult (ANum 3) (AMult (ANum 2) (ANum 1))) / empty_state 
+  (AMult (ANum 3) (AMult (ANum 2) (ANum 1))) / empty_state
   ==>a* e'.
 Proof.
-  (* FILL IN HERE *) Admitted.
+  eapply ex_intro.
+  normalize.
+  Admitted.
 (** [] *)
 
 
@@ -676,7 +737,7 @@ Proof.
 
 
 (** **** Exercise: 2 stars (variation1)  *)
-(** Suppose, that we add this new rule to the typing relation: 
+(** Suppose, that we add this new rule to the typing relation:
       | T_SuccBool : forall t,
            |- t \in TBool ->
            |- tsucc t \in TBool
@@ -693,7 +754,7 @@ Proof.
 [] *)
 
 (** **** Exercise: 2 stars (variation2)  *)
-(** Suppose, instead, that we add this new rule to the [step] relation: 
+(** Suppose, instead, that we add this new rule to the [step] relation:
       | ST_Funny1 : forall t2 t3,
            (tif ttrue t2 t3) ==> t3
    Which of the above properties become false in the presence of
@@ -713,7 +774,7 @@ Proof.
 
 (** **** Exercise: 2 stars, optional (variation4)  *)
 (** Suppose instead that we add this rule:
-      | ST_Funny3 : 
+      | ST_Funny3 :
           (tpred tfalse) ==> (tpred (tpred tfalse))
    Which of the above properties become false in the presence of
    this rule?  For each one that does, give a counter-example.
@@ -722,8 +783,8 @@ Proof.
 
 (** **** Exercise: 2 stars, optional (variation5)  *)
 (** Suppose instead that we add this rule:
-   
-      | T_Funny4 : 
+
+      | T_Funny4 :
             |- tzero \in TBool
    ]]
    Which of the above properties become false in the presence of
@@ -733,8 +794,8 @@ Proof.
 
 (** **** Exercise: 2 stars, optional (variation6)  *)
 (** Suppose instead that we add this rule:
-   
-      | T_Funny5 : 
+
+      | T_Funny5 :
             |- tpred tzero \in TBool
    ]]
    Which of the above properties become false in the presence of
@@ -754,7 +815,7 @@ Proof.
     might feel that it makes more sense for the predecessor of zero to
     be undefined, rather than being defined to be zero.  Can we
     achieve this simply by removing the rule from the definition of
-    [step]?  Would doing so create any problems elsewhere? 
+    [step]?  Would doing so create any problems elsewhere?
 
 (* FILL IN HERE *)
 [] *)
